Logic/Modal/Standard/Kripke/Geach/Definability.lean
@@ -8,147 +8,154 @@ namespace LO.Modal.Standard
 open System
 open System.Axioms (Geach)
 
+def GeachConfluent' (t : Geach.Taple) (R : α → α → Prop) := ∀ {x y z : α}, (RelItr R t.i x y) ∧ (RelItr R t.j x z) → ∃ u, (RelItr R t.m y u) ∧ (RelItr R t.n z u)
+
+namespace GeachConfluent'
+
+variable {R : α → α → Prop}
+
+@[simp]
+lemma serial_def : (GeachConfluent' ⟨0, 0, 1, 1⟩ R) ↔ Serial R := by simp [GeachConfluent', Symmetric]; aesop;
+
+@[simp]
+lemma reflexive_def : (GeachConfluent' ⟨0, 0, 1, 0⟩ R) ↔ Reflexive R := by simp [GeachConfluent', Reflexive];
+
+@[simp]
+lemma symmetric_def : (GeachConfluent' ⟨0, 1, 0, 1⟩ R) ↔ Symmetric R := by
+  simp [GeachConfluent', Symmetric]; aesop;
+
+@[simp]
+lemma transitive_def : (GeachConfluent' ⟨0, 2, 1, 0⟩ R) ↔ Transitive R := by simp [GeachConfluent', Transitive]; aesop;
+
+@[simp]
+lemma euclidean_def : (GeachConfluent' ⟨1, 1, 0, 1⟩ R) ↔ Euclidean R := by simp [GeachConfluent', Euclidean];
+
+@[simp]
+lemma confluent_def : (GeachConfluent' ⟨1, 1, 1, 1⟩ R) ↔ Confluent R := by simp [GeachConfluent', Confluent];
+
+@[simp]
+lemma extensive_def : (GeachConfluent' ⟨0, 1, 0, 0⟩ R) ↔ Extensive R := by
+  simp [GeachConfluent', Extensive];
+  constructor;
+  . intro h x y Rxy;
+    have := h rfl Rxy;
+    subst_vars;
+    trivial;
+  . intro h x y z Exy Rxz;
+    have := h Rxz;
+    subst_vars;
+    trivial;
+
+@[simp]
+lemma functional_def : (GeachConfluent' ⟨1, 1, 0, 0⟩ R) ↔ Functional R := by simp [GeachConfluent', Functional]; aesop
+
+@[simp]
+lemma dense_def : (GeachConfluent' ⟨0, 1, 2, 0⟩ R)  ↔ Dense R := by simp [GeachConfluent', Dense]; aesop;
+
+@[simp]
+lemma satisfies_eq : GeachConfluent' (α := α) t (· = ·) := by simp [GeachConfluent'];
+
+end GeachConfluent'
+
+
+def MultiGeachConfluent' (ts : List Geach.Taple) (R : α → α → Prop) : Prop :=
+  match ts with
+  | [] => True
+  | t :: ts => (GeachConfluent' t R) ∧ (MultiGeachConfluent' ts R)
+
+namespace MultiGeachConfluent'
+
+@[simp]
+lemma satisfies_eq : MultiGeachConfluent' (α := α) ts (· = ·) := by
+  induction ts <;> simp_all [MultiGeachConfluent'];
+
+end MultiGeachConfluent'
+
+
 namespace Kripke
+
+abbrev GeachConfluentFrameClass (t : Geach.Taple) (α) : FrameClass α := { F | (GeachConfluent' t) F }
+
+abbrev MultiGeachConfluentFrameClass (ts : List Geach.Taple) (α) : FrameClass α := { F | MultiGeachConfluent' ts F }
+
+@[simp]
+lemma MultiGeachConfluentFrameClass.def_nil : MultiGeachConfluentFrameClass [] α = AllFrameClass α := by
+  simp [MultiGeachConfluentFrameClass, MultiGeachConfluent']
+
+open Formula (atom kripke_satisfies)
+open Formula.kripke_satisfies (multibox_def multidia_def)
 
 variable [Inhabited α]
 
-def GeachConfluent (t : Geach.Taple) : FrameCondition α := λ F => ∀ {x y z : F}, (x ≺^[t.i] y) ∧ (x ≺^[t.j] z) → ∃ u, (y ≺^[t.m] u) ∧ (z ≺^[t.n] u)
-
-@[simp]
-def MultiGeachConfluent (ts : List Geach.Taple) : FrameCondition α :=
-  match ts with
-  | [] => λ _ => True
-  | t :: ts => λ F => (GeachConfluent t F) ∧ (MultiGeachConfluent ts F)
-
-namespace GeachConfluent
-
-variable {F : Frame α}
-
-@[simp] lemma serial_def : (GeachConfluent ⟨0, 0, 1, 1⟩ F) ↔ Serial F.Rel := by simp [GeachConfluent, Symmetric]; aesop;
-
-@[simp] lemma reflexive_def : (GeachConfluent ⟨0, 0, 1, 0⟩ F) ↔ Reflexive F.Rel := by simp [GeachConfluent, Reflexive];
-
-@[simp] lemma symmetric_def : (GeachConfluent ⟨0, 1, 0, 1⟩ F) ↔ Symmetric F.Rel := by simp [GeachConfluent, Symmetric]; aesop;
-
-@[simp] lemma transitive_def : (GeachConfluent ⟨0, 2, 1, 0⟩ F) ↔ Transitive F.Rel := by simp [GeachConfluent, Transitive]; aesop;
-
-@[simp] lemma euclidean_def : (GeachConfluent ⟨1, 1, 0, 1⟩ F) ↔ Euclidean F.Rel := by simp [GeachConfluent, Euclidean];
-
-@[simp] lemma confluent_def : (GeachConfluent ⟨1, 1, 1, 1⟩ F) ↔ Confluent F.Rel := by simp [GeachConfluent, Confluent];
-
-@[simp]
-lemma extensive_def : (GeachConfluent ⟨0, 1, 0, 0⟩ F) ↔ Extensive F.Rel := by
-  intros;
-  simp [GeachConfluent, Extensive];
-  constructor;
-  . intro h x y hyz;
-    have := h rfl hyz;
-    subst this;
-    trivial;
-  . intro h x y z hxy hxz;
-    have := h hxz;
-    subst hxy this;
-    trivial;
-
-@[simp] lemma functional_def : (GeachConfluent ⟨1, 1, 0, 0⟩ F) ↔ Functional F.Rel := by simp [GeachConfluent, Functional]; aesop
-
-@[simp] lemma dense_def : (GeachConfluent ⟨0, 1, 2, 0⟩ F)  ↔ Dense F.Rel := by simp [GeachConfluent, Dense]; aesop;
-
-lemma satisfies_TerminalFrame : GeachConfluent t (TerminalFrame α).toFrame := by simp [GeachConfluent, TerminalFrame.iff_relItr.mpr];
-
-end GeachConfluent
-
-
-namespace MultiGeachConfluent
-
-lemma satisfies_TerminalFrame : MultiGeachConfluent ts (TerminalFrame α).toFrame := by
-  induction ts with
-  | nil => simp;
-  | cons t ts ih =>
+instance {t : Geach.Taple} : 𝗴𝗲(t).DefinesKripkeFrameClass (GeachConfluentFrameClass t α) where
+  defines := by
+    intro F;
     constructor;
-    . exact GeachConfluent.satisfies_TerminalFrame;
-    . exact ih;
-
-end MultiGeachConfluent
-
-
-open Kripke
-open Formula
-open AxiomSet
-
-variable {Ax : AxiomSet α}
-
-instance AxiomSet.Geach.definability (t) : Definability (α := α) 𝗴𝗲(t) (GeachConfluent t) where
-  defines F := by
-    simp [AxiomSet.Geach, GeachConfluent];
-    constructor;
-    . intro h x y z hi hj;
+    . rintro h x y z ⟨hi, hj⟩;
+      simp at h;
       let M : Model α := { Frame := F, Valuation := λ v _ => y ≺^[t.m] v }
-      have him_x : kripke_satisfies M x (◇^[t.i](□^[t.m](Formula.atom default))) := by
+      have him_x : kripke_satisfies M x (◇^[t.i](□^[t.m](atom default))) := by
         apply kripke_satisfies.multidia_def.mpr;
         existsi y;
         constructor;
         . simpa;
         . apply kripke_satisfies.multibox_def.mpr; aesop;
-      have hjn_x : kripke_satisfies M x (□^[t.j](◇^[t.n]atom default)) := kripke_satisfies.mdp (h (Formula.atom default) M.Valuation x) him_x;
-      have hn_z : kripke_satisfies M z (◇^[t.n]atom default) := kripke_satisfies.multibox_def.mp hjn_x z hj;
+      have hjn_x : kripke_satisfies M x (□^[t.j](◇^[t.n](atom default))) := h (Formula.atom default) M.Valuation x him_x;
+      have hn_z : kripke_satisfies M z (◇^[t.n](atom default)) := kripke_satisfies.multibox_def.mp hjn_x z hj;
       obtain ⟨u, hzu, hyu⟩ := kripke_satisfies.multidia_def.mp hn_z;
       existsi u;
       exact ⟨hyu, hzu⟩;
-    . intro h p V x;
-      simp [AxiomSet.Geach];
-      intro y hxy hm z hxz;
-      obtain ⟨u, hyu, hzu⟩ := h hxy hxz;
+    . simp [AxiomSet.Geach, Axioms.Geach, kripke_satisfies];
+      intro h p V x him;
+      simp [multibox_def, multidia_def];
+      intro z rxz;
+      obtain ⟨y, rxy, hbp⟩ := multidia_def.mp him;
+      obtain ⟨u, ryu, rzu⟩ := h ⟨rxy, rxz⟩;
       use u;
       constructor;
       . assumption;
-      . exact hm u hyu;
+      . exact (multibox_def.mp hbp) _ ryu;
 
-instance AxiomSet.MultiGeach.definability (ts) : Definability (α := α) 𝗚𝗲(ts) (Kripke.MultiGeachConfluent ts) where
-  defines F := by
+instance {ts : List Geach.Taple} : 𝗚𝗲(ts).DefinesKripkeFrameClass (MultiGeachConfluentFrameClass ts α) where
+  defines := by
     induction ts with
-    | nil => apply AxiomSet.K.definability.defines;
+    | nil => simp;
     | cons t ts ih =>
-      simp only [MultiGeach.iff_cons, Semantics.RealizeSet.union_iff, MultiGeachConfluent];
+      have : 𝗴𝗲(t).DefinesKripkeFrameClass (GeachConfluentFrameClass t α) := inferInstance;
+      simp_all only [Semantics.RealizeSet.union_iff, AxiomSet.MultiGeach.iff_cons, MultiGeachConfluentFrameClass];
+      intro F;
       constructor;
       . rintro ⟨ht, hts⟩;
         constructor;
-        . exact AxiomSet.Geach.definability t |>.defines F |>.mp ht;
-        . apply ih.mp hts;
+        . exact this.defines.mp ht;
+        . simpa using hts;
       . rintro ⟨ht, hts⟩;
         constructor;
-        . exact AxiomSet.Geach.definability t |>.defines F |>.mpr ht;
-        . apply ih.mpr hts;
+        . exact this.defines.mpr ht;
+        . simpa using hts;
 
-variable {L : DeductionParameter α} [L.HasNec]
-
-instance instGeachDefinability [geach : L.IsGeach] : Definability Ax(L) (Kripke.MultiGeachConfluent geach.taples) := by
-  convert AxiomSet.MultiGeach.definability (α := α) geach.taples;
-  simp;
-
-instance : (𝔽ꟳ(𝗚𝗲(l)) : FiniteFrameClass α).IsNonempty where
+instance : (MultiGeachConfluentFrameClass ts α).IsNonempty where
   nonempty := by
     use (TerminalFrame α);
-    apply iff_definability_memAxiomSetFrameClass (AxiomSet.MultiGeach.definability l) |>.mpr;
-    exact MultiGeachConfluent.satisfies_TerminalFrame;
+    exact MultiGeachConfluent'.satisfies_eq;
 
-instance : FrameClass.IsNonempty (𝔽(𝗚𝗲(l)) : FrameClass α) := inferInstance
+instance : System.Consistent (𝐆𝐞(ts) : DeductionParameter α) := consistent (𝔽 := MultiGeachConfluentFrameClass ts α)
 
-instance : System.Consistent (𝐆𝐞(l) : DeductionParameter α) := inferInstance
-
-instance [geach : L.IsGeach] : FrameClass.IsNonempty 𝔽(Ax(L)) := by rw [geach.char]; infer_instance;
-
-instance [L.IsGeach] : System.Consistent L := inferInstance
+instance {Λ : DeductionParameter α} [geach : Λ.IsGeach] : System.Consistent Λ := by rw [geach.char]; infer_instance;
 
 instance : System.Consistent (𝐒𝟒 : DeductionParameter α) := inferInstance
 
 instance : System.Consistent (𝐒𝟓 : DeductionParameter α) := inferInstance
 
-instance : Definability (α := α) Ax(𝐒𝟒) (λ F => Reflexive F.Rel ∧ Transitive F.Rel) := by simpa using instGeachDefinability (L := 𝐒𝟒)
+/-
+abbrev PreorderFrameClass (α) : FrameClass α := { F | Reflexive F ∧ Transitive F }
+
+instance : Ax(𝐒𝟒).DefinesKripkeFrameClass (PreorderFrameClass α) := by simpa using instGeachDefinability (L := 𝐒𝟒)
 
 instance : Definability (α := α) Ax(𝐒𝟓) (λ F => Reflexive F.Rel ∧ Euclidean F.Rel) := by simpa using instGeachDefinability (L := 𝐒𝟓);
 
 instance : Definability (α := α) Ax(𝐓𝐫𝐢𝐯) (λ F => Reflexive F.Rel ∧ Extensive F.Rel) := by simpa using instGeachDefinability (L := 𝐓𝐫𝐢𝐯);
+-/
 
 end Kripke
 
