Logic/Modal/Standard/Kripke/Semantics.lean
@@ -13,11 +13,21 @@ def RelItr (R : α → α → Prop) : ℕ → α → α → Prop
   | 0 => (· = ·)
   | n + 1 => fun x y ↦ ∃ z, R x z ∧ RelItr R n z y
 
-@[simp]
-lemma relItr_zero {R : α → α → Prop} {x y : α} : RelItr R 0 x y ↔ x = y := iff_of_eq rfl
+namespace RelItr
 
 @[simp]
-lemma relItr_succ {R : α → α → Prop} {x y : α} : RelItr R (n + 1) x y ↔ ∃ z, R x z ∧ RelItr R n z y := iff_of_eq rfl
+lemma iff_zero {R : α → α → Prop} {x y : α} : RelItr R 0 x y ↔ x = y := iff_of_eq rfl
+
+@[simp]
+lemma iff_succ {R : α → α → Prop} {x y : α} : RelItr R (n + 1) x y ↔ ∃ z, R x z ∧ RelItr R n z y := iff_of_eq rfl
+
+@[simp]
+lemma eq : RelItr (α := α) (· = ·) n = (· = ·) := by
+  induction n with
+  | zero => rfl;
+  | succ n ih => aesop
+
+end RelItr
 
 namespace Kripke
 
@@ -34,25 +44,32 @@ instance (F : Frame α) : Nonempty F.World := F.World_nonempty
 
 instance : CoeSort (Frame α) (Type*) := ⟨Frame.World⟩
 
+instance : CoeFun (Frame α) (λ F => F.World → F.World → Prop) := ⟨Frame.Rel⟩
+
 instance : Coe (FiniteFrame α) (Frame α) := ⟨λ F ↦ F.toFrame⟩
 
 abbrev Frame.Rel' {F : Frame α} (w w' : F.World) := F.Rel w w'
 scoped infix:45 " ≺ " => Frame.Rel'
 
-protected abbrev Frame.RelItr (n : ℕ) {F : Frame α} (w w' : F.World) : Prop := RelItr (· ≺ ·) n w w'
-scoped notation w:45 " ≺^[" n "] " w':46 => Frame.RelItr n w w'
+protected abbrev Frame.RelItr' (n : ℕ) {F : Frame α} (w w' : F.World) : Prop := RelItr (· ≺ ·) n w w'
+scoped notation w:45 " ≺^[" n "] " w':46 => Frame.RelItr' n w w'
+
+
+protected def Frame.Finite (F : Frame α) := Finite F.World
+
 
 /-- Frame with single world and identiy relation -/
 abbrev TerminalFrame (α) : FiniteFrame α := { World := PUnit, Rel := (· = ·) }
 
 @[simp]
-lemma TerminalFrame.iff_rel : Frame.Rel' (F := (TerminalFrame α).toFrame) x y ↔ x = y := by aesop;
+lemma TerminalFrame.iff_rel' : Frame.Rel' (F := (TerminalFrame α).toFrame) x y ↔ x = y := by aesop;
 
 @[simp]
-lemma TerminalFrame.iff_relItr : Frame.RelItr n (F := (TerminalFrame α).toFrame) x y ↔ x = y := by
+lemma TerminalFrame.iff_relItr' : Frame.RelItr' n (F := (TerminalFrame α).toFrame) x y ↔ x = y := by
   induction n with
-  | zero => simp only [relItr_zero];
-  | succ n ih => simp_all only [relItr_succ, exists_eq_left', iff_true];
+  | zero => simp;
+  | succ n ih => simp_all; use x;
+
 
 abbrev FrameClass (α) := Set (Frame α)
 
@@ -72,8 +89,8 @@ class FiniteFrameClass.IsNonempty (𝔽 : FiniteFrameClass α) where
 def FrameClass.toFinite (𝔽 : FrameClass α) : FiniteFrameClass α := { F | ↑F ∈ 𝔽 }
 postfix:max "ꟳ" => FrameClass.toFinite
 
-instance : Coe (FrameClass α) (FiniteFrameClass α) := ⟨λ 𝔽 ↦ 𝔽ꟳ⟩
-
+-- instance : Coe (FrameClass α) (FiniteFrameClass α) := ⟨λ 𝔽 ↦ 𝔽ꟳ⟩
+instance : Coe (FiniteFrameClass α) (FrameClass α) := ⟨λ 𝔽 ↦ { ↑F | F ∈ 𝔽 }⟩
 
 abbrev FrameCondition (α) := Frame α → Prop
 
@@ -104,7 +121,7 @@ def Formula.kripke_satisfies (M : Kripke.Model α) (w : M.World) : Formula α �
   | and p q => (kripke_satisfies M w p) ∧ (kripke_satisfies M w q)
   | or p q  => (kripke_satisfies M w p) ∨ (kripke_satisfies M w q)
   | imp p q => (kripke_satisfies M w p) → (kripke_satisfies M w q)
-  | box p   => ∀ {w'}, w ≺ w' → (kripke_satisfies M w' p)
+  | box p   => ∀ {x}, w ≺ x → (kripke_satisfies M x p)
 
 namespace Formula.kripke_satisfies
 
@@ -116,6 +133,7 @@ variable {M : Model α} {w : M.World} {p q : Formula α}
 
 local infix:45 " ⊩ " => Formula.kripke_satisfies M
 
+/-
 @[simp] lemma atom_def : w ⊧ atom a ↔ M.Valuation w a := by simp [kripke_satisfies];
 @[simp] lemma top_def  : w ⊩ ⊤ ↔ True := by simp [kripke_satisfies];
 @[simp] lemma bot_def  : w ⊩ ⊥ ↔ False := by simp [kripke_satisfies];
@@ -124,9 +142,10 @@ local infix:45 " ⊩ " => Formula.kripke_satisfies M
 @[simp] lemma imp_def  : w ⊩ p ⟶ q ↔ w ⊩ p → w ⊩ q := by simp [kripke_satisfies, imp_iff_not_or];
 @[simp] lemma not_def  : w ⊩ ~p ↔ ¬w ⊩ p := by simp [kripke_satisfies];
 @[simp] lemma box_def  : w ⊩ □p ↔ ∀ w', w ≺ w' → w' ⊩ p := by simp [kripke_satisfies];
-@[simp] lemma dia_def  : w ⊩ ◇p ↔ ∃ w', w ≺ w' ∧ w' ⊩ p := by simp [kripke_satisfies];
+-/
 
-@[simp]
+lemma dia_def  : w ⊩ ◇p ↔ ∃ w', w ≺ w' ∧ w' ⊩ p := by simp [kripke_satisfies];
+
 lemma multibox_def : w ⊩ □^[n]p ↔ ∀ v, w ≺^[n] v → v ⊩ p := by
   induction n generalizing w with
   | zero => simp;
@@ -135,29 +154,29 @@ lemma multibox_def : w ⊩ □^[n]p ↔ ∀ v, w ≺^[n] v → v ⊩ p := by
     . intro h w' hww';
       simp at h;
       obtain ⟨v, hwv, hvw'⟩ := hww';
-      exact (ih.mp $ h _ hwv) w' hvw';
+      exact (ih.mp $ h hwv) w' hvw';
     . simp;
       intro h w' hww';
       apply ih.mpr;
       intro v hwv;
       exact h v w' hww' hwv;
 
-@[simp]
 lemma multidia_def : w ⊩ ◇^[n]p ↔ ∃ v, w ≺^[n] v ∧ v ⊩ p := by
   induction n generalizing w with
   | zero => simp;
   | succ n ih =>
     constructor;
     . intro h;
-      obtain ⟨v, hwv, hv⟩ := by simpa using h;
+      replace h : kripke_satisfies M w (◇◇^[n]p) := by simpa using h;
+      obtain ⟨v, hwv, hv⟩ := dia_def.mp h;
       obtain ⟨x, hvx, hx⟩ := ih.mp hv;
       existsi x;
       constructor;
       . existsi v; simp_all;
       . simpa;
-    . simp;
+    . simp [dia_def];
       intro x y hwy hyx hx;
-      existsi y;
+      use y;
       constructor;
       . simpa;
       . apply ih.mpr;
@@ -165,14 +184,12 @@ lemma multidia_def : w ⊩ ◇^[n]p ↔ ∃ v, w ≺^[n] v ∧ v ⊩ p := by
         simp_all;
 
 instance : Semantics.Tarski M.World where
-  realize_top := by simp [top_def];
-  realize_bot := by simp [bot_def];
-  realize_not := by simp [not_def];
-  realize_and := by simp [and_def];
-  realize_or  := by simp [or_def];
-  realize_imp := by simp [imp_def];
-
-lemma mdp (hpq : w ⊧ p ⟶ q) (hp : w ⊧ p) : w ⊧ q := imp_def.mp hpq hp
+  realize_top := by simp [kripke_satisfies];
+  realize_bot := by simp [kripke_satisfies];
+  realize_not := by simp [kripke_satisfies];
+  realize_and := by simp [kripke_satisfies];
+  realize_or  := by simp [kripke_satisfies];
+  realize_imp := by simp [kripke_satisfies];
 
 end Formula.kripke_satisfies
 
@@ -218,7 +235,7 @@ protected lemma mdp {F : Frame α} (hpq : F ⊧ p ⟶ q) (hp : F ⊧ p) : F ⊧ 
 
 end Formula.valid_on_KripkeFrame
 
-
+/-
 @[simp] def Formula.valid_on_FiniteKripkeFrame (F : FiniteFrame α) (f : Formula α) := (F.toFrame) ⊧ f
 namespace Formula.valid_on_FiniteKripkeFrame
 
@@ -227,7 +244,7 @@ protected instance semantics : Semantics (Formula α) (FiniteFrame α) := ⟨fun
 @[simp] protected lemma models_iff {F : FiniteFrame α} : F ⊧ f ↔ valid_on_FiniteKripkeFrame F f := iff_of_eq rfl
 
 end Formula.valid_on_FiniteKripkeFrame
-
+-/
 
 @[simp] def Formula.valid_on_KripkeFrameClass (𝔽 : FrameClass α) (p : Formula α) := ∀ F ∈ 𝔽, F ⊧ p
 
@@ -256,7 +273,7 @@ protected lemma mdp (hpq : 𝔽 ⊧ p ⟶ q) (hp : 𝔽 ⊧ p) : 𝔽 ⊧ q := b
 
 end Formula.valid_on_KripkeFrameClass
 
-
+/-
 @[simp] def Formula.valid_on_FiniteKripkeFrameClass (𝔽 : FiniteFrameClass α) (p : Formula α) := ∀ F ∈ 𝔽, F ⊧ p
 
 namespace Formula.valid_on_FiniteKripkeFrameClass
@@ -266,32 +283,10 @@ protected instance : Semantics (Formula α) (FiniteFrameClass α) := ⟨fun 𝔽
 @[simp] protected lemma models_iff {𝔽 : FiniteFrameClass α} : 𝔽 ⊧ f ↔ Formula.valid_on_FiniteKripkeFrameClass 𝔽 f := iff_of_eq rfl
 
 end Formula.valid_on_FiniteKripkeFrameClass
-
-/-
-def AxiomSet.KripkeFrameClass (Ax : AxiomSet α) : FrameClass α := { F | F ⊧* System.theory (DeductionParameter.Normal Ax) }
-notation "𝔽₂(" Ax ")" => AxiomSet.KripkeFrameClass Ax
-
-def AxiomSet.FiniteKripkeFrameClass (Ax : AxiomSet α) : FiniteFrameClass α := { F | F ⊧* System.theory (DeductionParameter.Normal Ax)  }
-notation "𝔽₂ꟳ(" Ax ")" => AxiomSet.FiniteKripkeFrameClass Ax
-
-
-def DeductionParamter.KripkeFrameClass (𝓓 : DeductionParameter α) [𝓓.IsNormal] : FrameClass α := { F | F ⊧* System.theory 𝓓 }
-notation "𝔽(" 𝓓 ")" => DeductionParamter.KripkeFrameClass 𝓓
-
-def DeductionParamter.FiniteKripkeFrameClass (𝓓 : DeductionParameter α) [𝓓.IsNormal] : FiniteFrameClass α := { F | F ⊧* System.theory 𝓓 }
-notation "𝔽ꟳ(" 𝓓 ")" => DeductionParamter.FiniteKripkeFrameClass 𝓓
-
-
-def Kripke.AxiomSetFrameClass (Ax : AxiomSet α) : FrameClass α := { (F : Frame α) | F ⊧* Ax }
-notation "𝔽(" Ax ")" => Kripke.AxiomSetFrameClass Ax
-
-def Kripke.AxiomSetFiniteFrameClass (Ax : AxiomSet α) : FiniteFrameClass α := { (F : FiniteFrame α) | F.toFrame ⊧* Ax }
-notation "𝔽ꟳ(" Ax ")" => Kripke.AxiomSetFiniteFrameClass Ax
 -/
 
-
 class AxiomSet.DefinesKripkeFrameClass (Ax : AxiomSet α) (𝔽 : FrameClass α) where
-  defines : ∀ {F : Frame α}, F ⊧* Ax ↔ F ∈ 𝔽
+  defines : ∀ {F}, F ⊧* Ax ↔ F ∈ 𝔽
 
 instance AxiomSet.DefinesKripkeFrameClass.union
   {Ax₁ Ax₂ : AxiomSet α}
@@ -310,117 +305,39 @@ instance AxiomSet.DefinesKripkeFrameClass.union
       . apply definability₁.defines.mpr h₁;
       . apply definability₂.defines.mpr h₂;
 
+
+class AxiomSet.DefinesFiniteKripkeFrameClass (Ax : AxiomSet α) (𝔽 : FiniteFrameClass α) where
+  defines : ∀ {F : FiniteFrame α}, (F : Frame α) ⊧* Ax ↔ F ∈ 𝔽
+
+instance AxiomSet.DefinesFiniteKripkeFrameClass.union
+  {Ax₁ Ax₂ : AxiomSet α}
+  (definability₁ : Ax₁.DefinesFiniteKripkeFrameClass 𝔽₁) (definability₂ : Ax₂.DefinesFiniteKripkeFrameClass 𝔽₂)
+  : (Ax₁ ∪ Ax₂).DefinesFiniteKripkeFrameClass (𝔽₁ ∩ 𝔽₂) where
+  defines := by
+    intro F;
+    simp only [Semantics.RealizeSet.union_iff];
+    constructor;
+    . intro ⟨h₁, h₂⟩;
+      constructor;
+      . exact definability₁.defines.mp h₁;
+      . exact definability₂.defines.mp h₂;
+    . intro ⟨h₁, h₂⟩;
+      constructor;
+      . apply definability₁.defines.mpr h₁;
+      . apply definability₂.defines.mpr h₂;
+
 open Formula
 
 namespace Kripke
-
-def ConditionalFrameClass (P : FrameCondition α) : FrameClass α := { F | P F }
-notation "𝔽(" P ")" => ConditionalFrameClass P
-
-def ConditionalFiniteFrameClass (P : FiniteFrameCondition α) : FiniteFrameClass α := { F | P F }
-notation "𝔽ꟳ(" P ")" => ConditionalFiniteFrameClass P
-
 
 abbrev AllFrameClass (α) : FrameClass α := Set.univ
 
 instance : (AllFrameClass α).IsNonempty where
   nonempty := by use TerminalFrame α; trivial;
 
-
-abbrev TransitiveFrameClass (α) : FrameClass α := 𝔽(λ F => Transitive F.Rel)
-
 instance : 𝗞.DefinesKripkeFrameClass (AllFrameClass α) where
   defines := by simp only [Set.mem_univ, iff_true]; apply valid_on_KripkeFrame.axiomK;
 
 end Kripke
-
-/-
-lemma validOnAxiomSetFrameClass_axiom (h : p ∈ Ax) : 𝔽(Ax) ⊧ p := by intro F hF; exact hF.realize h;
-
-/-- Every frame that valid all axioms in `Ax` satisfy frame property `P` -/
-class Definability (Ax : AxiomSet α) (P : FrameCondition α) where
-  defines : ∀ (F : Frame α), F ⊧* Ax ↔ P F
-
-instance Definability.union (definability₁ : Definability Ax₁ P₁) (definability₂ : Definability Ax₂ P₂) : Definability (Ax₁ ∪ Ax₂) (λ F => P₁ F ∧ P₂ F) where
-  defines F := by
-    constructor;
-    . intro h;
-      simp only [Semantics.RealizeSet.union_iff] at h;
-      constructor;
-      . exact Definability.defines F |>.mp h.1;
-      . exact Definability.defines F |>.mp h.2;
-    . intro h;
-      simp only [Semantics.RealizeSet.union_iff];
-      constructor;
-      . apply Definability.defines F |>.mpr h.1;
-      . apply Definability.defines F |>.mpr h.2;
-
-lemma iff_definability_memAxiomSetFrameClass (definability : Definability Ax P) : ∀ {F : Frame α}, F ∈ 𝔽(Ax) ↔ P F := by
-  apply definability.defines;
-
-
-/-- Every **finite** frame that valid all axioms in `Ax` satisfy **finite** frame property `P` -/
-class FiniteDefinability (Ax : AxiomSet α) (P : FiniteFrameCondition α) where
-  fin_defines : ∀ (F : FiniteFrame α), F.toFrame ⊧* Ax ↔ P F
-
-instance FiniteDefinability.union (definability₁ : FiniteDefinability Ax₁ P₁) (definability₂ : FiniteDefinability Ax₂ P₂) : FiniteDefinability (Ax₁ ∪ Ax₂) (λ F => P₁ F ∧ P₂ F) where
-  fin_defines F := by
-    constructor;
-    . intro h;
-      simp only [Semantics.RealizeSet.union_iff] at h;
-      constructor;
-      . exact FiniteDefinability.fin_defines F |>.mp h.1;
-      . exact FiniteDefinability.fin_defines F |>.mp h.2;
-    . intro h;
-      simp only [Semantics.RealizeSet.union_iff];
-      constructor;
-      . apply FiniteDefinability.fin_defines F |>.mpr h.1;
-      . apply FiniteDefinability.fin_defines F |>.mpr h.2;
-
-lemma iff_finiteDefinability_memFiniteFrameClass (definability : FiniteDefinability Ax P) : ∀ {F : FiniteFrame α}, 𝔽ꟳ(Ax) F ↔ P F := by
-  apply definability.fin_defines;
-
-instance [definability : Definability Ax P] : FiniteDefinability Ax (λ F => P F.toFrame) where
-  fin_defines F := by
-    constructor;
-    . exact iff_definability_memAxiomSetFrameClass definability |>.mp;
-    . exact iff_definability_memAxiomSetFrameClass definability |>.mpr;
-
-instance [ne : 𝔽ꟳ.IsNonempty] : 𝔽.IsNonempty where
-  nonempty := by obtain ⟨F, hF⟩ := ne.nonempty; existsi F; exact hF;
-
-instance [ne : 𝔽ꟳ(Ax).IsNonempty ] : 𝔽(Ax).IsNonempty where
-  nonempty := by obtain ⟨F, hF⟩ := ne.nonempty; existsi F; exact hF;
-
-end Kripke
-
-section K
-
-instance AxiomSet.K.definability : Definability (α := α) 𝗞 (λ _ => True) where
-  defines := by
-    simp [valid_on_KripkeFrame, valid_on_KripkeModel, System.Axioms.K];
-    intros; subst_vars;
-    simp_all;
-
-instance AxiomSet.K.finiteDefinability : FiniteDefinability (α := α) 𝗞 (λ _ => True) where
-  fin_defines := by
-    simp [valid_on_KripkeFrame, valid_on_KripkeModel, System.Axioms.K];
-    intros; subst_vars;
-    simp_all;
-
-instance [definability : Definability Ax P] : Definability (𝗞 ∪ Ax) P := by simpa using Definability.union AxiomSet.K.definability definability;
-
-instance [definability : FiniteDefinability Ax P] : FiniteDefinability (𝗞 ∪ Ax) P := by simpa using FiniteDefinability.union AxiomSet.K.finiteDefinability definability;
-
-instance : (𝔽ꟳ(𝗞) : FiniteFrameClass α).IsNonempty where
-  nonempty := by
-    existsi TerminalFrame α;
-    apply iff_finiteDefinability_memFiniteFrameClass AxiomSet.K.finiteDefinability |>.mpr;
-    trivial;
-
-instance : (𝔽(𝗞) : FrameClass α).IsNonempty  := inferInstance
-
-end K
--/
 
 end LO.Modal.Standard
