Logic/Modal/Standard/Kripke/Ver.lean
@@ -3,48 +3,44 @@ import Logic.Modal.Standard.Kripke.Completeness
 
 namespace LO.Modal.Standard
 
+namespace Kripke
+
 open System
 open Kripke
 open Formula
 
 variable {α} [Inhabited α] [DecidableEq α]
 
-instance AxiomSet.Ver.definability : Definability (α := α) 𝗩𝗲𝗿 (λ F => Isolated F.Rel) where
+abbrev IsolatedFrameClass (α) : FrameClass α := { F | Isolated F }
+
+instance : 𝗩𝗲𝗿.DefinesKripkeFrameClass (IsolatedFrameClass α) where
   defines := by
     simp [valid_on_KripkeFrame, valid_on_KripkeModel, Isolated];
     intro F;
     constructor;
     . intro h x y hxy;
-      exact h ⊥ (λ _ _ => True) x y hxy;
-    . intros;
+      exact h ⊥ (λ _ _ => True) x hxy;
+    . intro hIrrefl p V x y hxy;
       simp_all;
 
-instance Ver.definability : Definability (α := α) Ax(𝐕𝐞𝐫) (λ F => Isolated F.Rel) := by
-  simpa using Definability.union AxiomSet.K.definability AxiomSet.Ver.definability
-
-instance : (𝔽ꟳ(Ax(𝐕𝐞𝐫)) : FiniteFrameClass α).IsNonempty where
+instance : (IsolatedFrameClass α).IsNonempty where
   nonempty := by
     use { World := PUnit, Rel := (· ≠ ·) };
-    apply iff_definability_memAxiomSetFrameClass (Ver.definability) |>.mpr;
-    simp_all [Isolated];
+    simp [Isolated];
 
-namespace Kripke
+open DeductionParameter (Normal)
 
-open MaximalConsistentTheory
+instance : System.Consistent (𝐕𝐞𝐫 : DeductionParameter α) := consistent (𝔽 := IsolatedFrameClass α)
 
-lemma definability_canonicalFrame_Ver {𝓓 : DeductionParameter α} [𝓓.IsNormal] [Inhabited (𝓓)-MCT] (hAx : 𝗩𝗲𝗿 ⊆ Ax(𝓓))
-  : Isolated (CanonicalFrame 𝓓).Rel := by
-  intro x y hxy;
-  have : 𝓓 ⊢! □⊥ := ⟨Deduction.maxm (Set.mem_of_subset_of_mem hAx (by simp))⟩
-  have := iff_valid_on_canonicalModel_deducible.mpr this x y hxy;
+lemma isolated_Ver_CanonicalFrame : (CanonicalFrame 𝗩𝗲𝗿) ∈ IsolatedFrameClass α := by
+  intro x y rxy;
+  have : (CanonicalModel (α := α) 𝗩𝗲𝗿) ⊧ □⊥ := iff_valid_on_canonicalModel_deducible.mpr $ axiomVer!;
+  simp [valid_on_KripkeModel, kripke_satisfies] at this;
+  obtain ⟨p, ⟨hx, hy⟩⟩ := @this x y;
+  have := rxy hx;
   contradiction;
 
-instance : Canonical (𝐕𝐞𝐫 : DeductionParameter α) := by
-  apply canonical_of_definability Ver.definability;
-  apply definability_canonicalFrame_Ver;
-  simp;
-
-instance : Complete (𝐕𝐞𝐫 : DeductionParameter α) 𝔽(Ax(𝐕𝐞𝐫)) := instComplete
+instance : Complete (𝐕𝐞𝐫 : DeductionParameter α) (IsolatedFrameClass α) := instComplete_of_mem_canonicalFrame isolated_Ver_CanonicalFrame
 
 end Kripke
 
