Logic/Modal/Standard/Kripke/GL.lean
@@ -1,42 +1,45 @@
 import Logic.Vorspiel.BinaryRelations
-import Logic.Modal.Standard.Kripke.Semantics
 import Logic.Modal.Standard.Kripke.Soundness
 
 namespace LO.Modal.Standard
 
-variable {W α : Type u} [Inhabited W] [Inhabited α]
+namespace Kripke
 
 open System
 open Kripke
 open Formula
 
+variable {α : Type u} [Inhabited α]
+
 variable {F : Kripke.Frame α}
 
-private lemma AxiomSet.L.definability.implies_transitive : F ⊧* 𝗟 → Transitive F.Rel := by
+abbrev TransitiveCWFFrameClass (α) : FrameClass α := { F | Transitive F ∧ ConverseWellFounded F }
+
+private lemma trans_of_L : F ⊧* 𝗟 → Transitive F.Rel := by
   contrapose;
   intro hT; simp [Transitive] at hT;
   obtain ⟨w₁, w₂, r₁₂, w₃, r₂₃, nr₁₃⟩ := hT;
-  simp [valid_on_KripkeFrame, valid_on_KripkeFrame, valid_on_KripkeModel];
-  existsi (atom default), (λ w' _ => w' ≠ w₂ ∧ w' ≠ w₃), w₁;
+  simp [valid_on_KripkeFrame, valid_on_KripkeFrame, valid_on_KripkeModel, kripke_satisfies];
+  use (atom default), (λ w' _ => w' ≠ w₂ ∧ w' ≠ w₃), w₁;
   constructor;
   . intro x hx h;
     by_cases hx₂ : x = w₂;
-    . subst hx₂; simpa [kripke_satisfies] using h w₃ r₂₃;
+    . subst hx₂; simpa [kripke_satisfies] using h r₂₃;
     . by_cases hx₃ : x = w₃ <;> simp_all [kripke_satisfies, hx₃];
   . existsi w₂; simpa [kripke_satisfies];
 
-private lemma AxiomSet.L.definability.implies_cwf  : F ⊧* 𝗟 → ConverseWellFounded F.Rel := by
+private lemma cwf_of_L  : F ⊧* 𝗟 → ConverseWellFounded F.Rel := by
   contrapose;
   intro hCF;
   obtain ⟨X, hX₁, hX₂⟩ := by simpa using ConverseWellFounded.iff_has_max.not.mp hCF;
-  simp [valid_on_KripkeFrame, valid_on_KripkeFrame, valid_on_KripkeModel];
-  existsi (atom default), (λ w _ => w ∉ X), hX₁.some;
+  simp [valid_on_KripkeFrame, valid_on_KripkeFrame, valid_on_KripkeModel, kripke_satisfies];
+  use (atom default), (λ w _ => w ∉ X), hX₁.some;
   constructor;
   . intro x _;
     by_cases hxs : x ∈ X
     . obtain ⟨y, hy₁, hy₂⟩ := hX₂ x hxs;
       intro h;
-      exact h x (by simp_all only [kripke_satisfies]);
+      exact h (by simp_all only [kripke_satisfies]);
     . aesop;
   . obtain ⟨w', hw'₁, hw'₂⟩ := hX₂ hX₁.some (by apply Set.Nonempty.some_mem);
     existsi w';
@@ -44,24 +47,61 @@ private lemma AxiomSet.L.definability.implies_cwf  : F ⊧* 𝗟 → ConverseWel
     . simpa using hw'₂;
     . simpa [kripke_satisfies];
 
-private lemma AxiomSet.L.definability.impliedby : (Transitive F.Rel ∧ ConverseWellFounded F.Rel) → F ⊧* 𝗟 := by
+private lemma L_of_trans_and_cwf : (Transitive F.Rel ∧ ConverseWellFounded F.Rel) → F ⊧* 𝗟 := by
   rintro ⟨hTrans, hWF⟩;
   simp [AxiomSet.L, Axioms.L];
   intro p V w;
   simp [kripke_satisfies];
-  contrapose;
+  contrapose; push_neg;
   intro h;
-  obtain ⟨z, rwz, hz⟩ := by simpa using h;
-  obtain ⟨xm, ⟨hxm₁, hxm₂⟩⟩ := hWF.has_min ({ x | (F.Rel w x) ∧ ¬(kripke_satisfies ⟨F, V⟩ x p) }) (by existsi z; simp_all)
-  simp;
-  existsi xm;
-  have : kripke_satisfies ⟨F, V⟩ xm (□p) := by
-    by_contra hC;
-    obtain ⟨y, hy₁, hy₂⟩ := by simpa using hC;
-    have : ¬(xm ≺ y) := hxm₂ y ⟨(hTrans (by simp_all) hy₁), hy₂⟩;
-    contradiction;
-  simp_all;
+  obtain ⟨z, rwz, hz⟩ := h;
+  obtain ⟨m, ⟨⟨rwm, hm⟩, hm₂⟩⟩ := hWF.has_min ({ x | (F.Rel w x) ∧ ¬(kripke_satisfies ⟨F, V⟩ x p) }) (by use z; simp_all)
+  use m;
+  constructor;
+  . exact rwm;
+  . constructor;
+    . simp [flip] at hm₂;
+      intro n rmn;
+      apply not_imp_not.mp $ hm₂ n (hTrans rwm rmn);
+      exact rmn;
+    . exact hm;
 
+instance instLDefines : 𝗟.DefinesKripkeFrameClass (TransitiveCWFFrameClass α) where
+  defines := by
+    intro F;
+    constructor;
+    . intro h;
+      constructor;
+      . exact trans_of_L h;
+      . exact cwf_of_L h;
+    . exact L_of_trans_and_cwf;
+
+abbrev TransitiveIrreflexiveFiniteFrameClass (α) : FiniteFrameClass α := { F | Transitive F.toFrame ∧ Irreflexive F.toFrame }
+
+instance : 𝗟.DefinesFiniteKripkeFrameClass (TransitiveIrreflexiveFiniteFrameClass α) where
+  defines := by
+    intro F;
+    constructor;
+    . intro h;
+      obtain ⟨hTrans, hCWF⟩ := instLDefines.defines.mp h;
+      constructor;
+      . exact hTrans;
+      . by_contra hC; simp [Irreflexive] at hC;
+        obtain ⟨w, h⟩ := hC;
+        have := ConverseWellFounded.iff_has_max.mp hCWF {w} (by simp);
+        simp_all;
+    . rintro ⟨hTrans, hIrrefl⟩;
+      apply instLDefines.defines.mpr;
+      exact ⟨hTrans, Finite.converseWellFounded_of_trans_irrefl' F.World_finite hTrans hIrrefl⟩;
+
+
+instance : (TransitiveIrreflexiveFiniteFrameClass α).IsNonempty where
+  nonempty := by
+    use { World := PUnit, Rel := (· ≠ ·) };
+    simp [Transitive, Irreflexive];
+
+
+/-
 open AxiomSet.L.definability in
 instance AxiomSet.L.definability : Definability (α := α) 𝗟 (λ F => Transitive F.Rel ∧ ConverseWellFounded F.Rel) where
   defines F := by
@@ -106,5 +146,8 @@ instance : (𝔽ꟳ(Ax(𝐆𝐋)) : FiniteFrameClass α).IsNonempty where
     simp [Transitive, Irreflexive];
 
 instance instGLConsistencyViaFrameClassNonemptiness : System.Consistent (𝐆𝐋 : DeductionParameter α) := inferInstance
+-/
+
+end Kripke
 
 end LO.Modal.Standard
