Logic/Modal/Standard/Kripke/Soundness.lean
@@ -11,7 +11,7 @@ open Formula
 open DeductionParameter (Normal)
 
 lemma sound [definability : Ax.DefinesKripkeFrameClass 𝔽] (d : (Normal Ax) ⊢! p) : 𝔽 ⊧ p := by
-  induction d using Deduction.inducition_with_nec! with
+  induction d using Deduction.inducition_with_necOnly! with
   | hMaxm h =>
     simp only [Set.mem_setOf_eq] at h;
     rcases h with (hK | hR);
@@ -21,12 +21,12 @@ lemma sound [definability : Ax.DefinesKripkeFrameClass 𝔽] (d : (Normal Ax) �
   | hMdp ihpq ihp => exact valid_on_KripkeFrameClass.mdp ihpq ihp;
   | hNec ih => exact valid_on_KripkeFrameClass.nec ih;
   | hDisj₃ =>
-    simp_all [valid_on_KripkeFrameClass, valid_on_KripkeFrame, valid_on_KripkeModel];
+    simp_all [valid_on_KripkeFrameClass, valid_on_KripkeFrame, valid_on_KripkeModel, kripke_satisfies];
     intros; rename_i hpr hqr hpq;
     cases hpq with
     | inl hp => exact hpr hp;
     | inr hq => exact hqr hq;
-  | _ => simp_all [valid_on_KripkeFrameClass, valid_on_KripkeFrame, valid_on_KripkeModel];
+  | _ => simp_all [valid_on_KripkeFrameClass, valid_on_KripkeFrame, valid_on_KripkeModel, kripke_satisfies];
 
 instance instSound [Ax.DefinesKripkeFrameClass 𝔽] : Sound (DeductionParameter.Normal Ax) 𝔽 := ⟨sound⟩
 
@@ -42,46 +42,11 @@ lemma consistent (𝔽 : FrameClass α) [Ax.DefinesKripkeFrameClass 𝔽] [𝔽.
   apply System.Consistent.of_unprovable;
   exact unprovable_bot 𝔽;
 
-instance : System.Consistent (𝐊 : DeductionParameter α) := by
-  simpa [←Normal.isK] using consistent (Ax := 𝗞) (𝔽 := AllFrameClass α)
+private instance instConsistent_of_K' : System.Consistent ((Normal 𝗞) : DeductionParameter α) := consistent (𝔽 := AllFrameClass α)
 
-/-
-lemma sound_on_frameclass (d : L ⊢ p) : 𝔽(Ax(L)) ⊧ p := by
-  induction d using Deduction.inducition_with_nec with
-  | hMaxm h => exact validOnAxiomSetFrameClass_axiom h;
-  | hMdp _ _ ihpq ihp =>
-    intro F hF V w;
-    exact (ihpq F hF V w) (ihp F hF V w);
-  | hNec _ ih =>
-    intro F hF V w w' _;
-    exact ih F hF V w';
-  | hDisj₃ =>
-    simp_all [valid_on_KripkeFrameClass, valid_on_KripkeFrame, valid_on_KripkeModel];
-    intros; rename_i hpr hqr hpq;
-    cases hpq with
-    | inl hp => exact hpr hp;
-    | inr hq => exact hqr hq;
-  | _ => simp_all [valid_on_KripkeFrameClass, valid_on_KripkeFrame, valid_on_KripkeModel];
+instance instConsistent_of_K : System.Consistent (𝐊 : DeductionParameter α) := by
+  simpa [←Normal.isK] using instConsistent_of_K';
 
-lemma sound!_on_frameclass : L ⊢! p → 𝔽(Ax(L)) ⊧ p := λ ⟨d⟩ => sound_on_frameclass d
 
-instance : Sound L 𝔽(L.axiomSet) := ⟨sound!_on_frameclass⟩
-
-lemma unprovable_bot [ne : 𝔽(Ax(L)).IsNonempty] : L ⊬! ⊥ := by
-  intro h;
-  obtain ⟨F, hF⟩ := ne.nonempty;
-  simpa using sound!_on_frameclass h F hF;
-
-instance Consistent_of_nonemptyFrameClass [𝔽(Ax(L)).IsNonempty] : System.Consistent L := System.Consistent.of_unprovable $ unprovable_bot
-
-lemma unprovable_bot_finite [ne : 𝔽ꟳ(Ax(L)).IsNonempty] : L ⊬! ⊥ := by
-  intro h;
-  obtain ⟨F, hF⟩ := ne.nonempty;
-  simpa using sound!_on_frameclass h F.toFrame hF;
-
-instance Consistent_of_nonemptyFiniteFrameClass [𝔽ꟳ(Ax(L)).IsNonempty] : System.Consistent L := System.Consistent.of_unprovable $ unprovable_bot_finite
-
-instance : System.Consistent (𝐊 : DeductionParameter α) := inferInstance
--/
 
 end LO.Modal.Standard.Kripke
